strlen_proofs.v
@@ -1,15 +1,20 @@
-(* Example proofs using CoqBAP for Intel x86 Architecture
- *
- * Copyright (c) 2018 Kevin W. Hamlen
- * Computer Science Department
- * The University of Texas at Dallas
- *
- * Any use, commercial or otherwise, requires the express permission of
- * the author.
- *
- * To run this module, first load the BapSyntax, BapInterp, BapStatics,
- * Bap_i386, and strlen_i386 modules, and compile each (in that order)
- * using menu option Compile->Compile buffer.
+(* Example proofs using Picinae for Intel x86 Architecture
+
+   Copyright (c) 2018 Kevin W. Hamlen
+   Computer Science Department
+   The University of Texas at Dallas
+
+   Any use, commercial or otherwise, requires the express permission of
+   the author.
+
+   To run this module, first load and compile:
+   * Picinae_syntax
+   * Picinae_theory
+   * Picinae_statics
+   * Picinae_i386
+   * strlen_i386
+   (in that order) and then compile this module using menu option
+   Compile->Compile buffer.
  *)
 
 Require Import Utf8.
@@ -17,28 +22,28 @@ Require Import FunctionalExtensionality.
 Require Import Arith.
 Require Import NArith.
 Require Import ZArith.
-Require Import Bap_i386.
+Require Import Picinae_i386.
 Require Import strlen_i386.
 
-Import BAPx86.
+Import Picinae_x86.
 Import X86Notations.
 Open Scope N.
 
 
 (* Example #1: Type safety
-   We first prove that the program is well-typed (automated by the BAP_typecheck tactic).
+   We first prove that the program is well-typed (automated by the Picinae_typecheck tactic).
    This is useful for later inferring that all CPU registers and memory contents have
    values of appropriate bitwidth throughout the program's execution. *)
 Theorem strlen_welltyped: welltyped_prog x86typctx strlen_i386.
 Proof.
-  BAP_typecheck.
+  Picinae_typecheck.
 Qed.
 
 (* Example #2: Memory safety
    Strlen contains no memory-writes, and is therefore trivially memory-safe. *)
 Theorem strlen_preserves_memory:
-  forall RW s m n s' x,
-  exec_prog RW strlen_i386 0 s m n s' x -> s' V_MEM32 = s V_MEM32.
+  forall s m n s' x,
+  exec_prog strlen_i386 0 s m n s' x -> s' V_MEM32 = s V_MEM32.
 Proof.
   intros. eapply prog_noassign_inv; [|exact H].
   intro a. destruct a as [|a]. discriminate 1.
@@ -70,8 +75,17 @@ Qed.
    and it restores ESP on exit. *)
 
 Theorem strlen_preserves_ebx:
-  forall RW s m n s' x,
-  exec_prog RW strlen_i386 0 s m n s' x -> s' R_EBX = s R_EBX.
+  forall s m n s' x,
+  exec_prog strlen_i386 0 s m n s' x -> s' R_EBX = s R_EBX.
+Proof.
+  intros. eapply prog_noassign_inv; [|exact H].
+  intro a. destruct a as [|a]. discriminate 1.
+  repeat first [ exact I | destruct a as [a|a|] | simpl; (repeat split); discriminate 1 ].
+Qed.
+
+Theorem strlen_preserves_readable:
+  forall s m n s' x,
+  exec_prog strlen_i386 0 s m n s' x -> s' A_READ = s A_READ.
 Proof.
   intros. eapply prog_noassign_inv; [|exact H].
   intro a. destruct a as [|a]. discriminate 1.
@@ -95,10 +109,10 @@ Proof.
 Qed.
 
 Theorem strlen_preserves_esp:
-  forall RW s esp mem m n s' x
+  forall s esp mem m n s' x
          (ESP0: s R_ESP = Some (VaN esp 32)) (MEM0: s V_MEM32 = Some (VaM mem 32))
          (RET: strlen_i386 (getmem LittleE 4 mem esp) = None)
-         (XP: exec_prog RW strlen_i386 0 s m n s' x),
+         (XP: exec_prog strlen_i386 0 s m n s' x),
   strlen_esp_inv esp mem x s'.
 Proof.
   intros. pattern x,s',n.
@@ -120,7 +134,7 @@ Proof.
   ).
 
   destruct (fin_dec x1) as [FIN|FIN]. subst x1. exact I.
-  stock_store in XS. simpl_stmt in XS; [|assumption]. destruct XS. subst x1.
+  stock_store in XS. x86_simpl_stmt in XS; [|assumption]. destruct XS. subst x1.
   unfold strlen_esp_inv. destruct (N.eq_dec _ _).
     exact I.
     contradict n. reflexivity.
@@ -681,13 +695,13 @@ Definition strlen_inv (mem:addr->N) (esp:N) :=
   x86_subroutine_inv strlen_i386 (strlen_inv_set mem esp) (strlen_postcond mem esp) (getmem LittleE 4 mem esp).
 
 Theorem strlen_partial_correctness:
-  forall RW s esp mem m n s' x
-         (HI: ~ RW false mem 32 (2^32 - 1)%N)
+  forall s esp mem m n s' x
+         (HI0: ~ mem_readable s (2^32 - 1)%N)
          (MDL0: models x86typctx s)
          (ESPLO: esp + 8 <= 2^32)
          (ESP0: s R_ESP = Some (VaN esp 32)) (MEM0: s V_MEM32 = Some (VaM mem 32))
          (RET: strlen_i386 (getmem LittleE 4 mem esp) = None)
-         (XP0: exec_prog RW strlen_i386 0 s m n s' x),
+         (XP0: exec_prog strlen_i386 0 s m n s' x),
   match strlen_inv mem esp x s' n with Some P => P | None => True end.
 Proof.
   intros.
@@ -697,12 +711,15 @@ Proof.
   intros.
   assert (MEM: s1 V_MEM32 = Some (VaM mem 32)).
     rewrite <- MEM0. eapply strlen_preserves_memory. exact XP.
+  assert (HI: ~ mem_readable s1 (2^32 - 1)%N).
+    unfold mem_readable. intro H. destruct H as [r [H1 H2]]. apply HI0. exists r. split; [|exact H2].
+    erewrite <- strlen_preserves_readable; eassumption.
   assert (ESP: strlen_esp_inv esp mem (Exit a1) s1).
     eapply strlen_preserves_esp. exact ESP0. exact MEM0. exact RET. exact XP.
   assert (MDL: models x86typctx s1).
     eapply preservation_exec_prog. exact MDL0. apply strlen_welltyped. exact XP.
   unfold strlen_esp_inv in ESP. unfold strlen_inv, x86_subroutine_inv in PRE.
-  clear s MDL0 MEM0 ESP0 XP XP0.
+  clear s HI0 MDL0 MEM0 ESP0 XP XP0.
   assert (WTM:=x86_wtm MDL MEM). simpl in WTM.
 
   destruct (N.eq_dec a1 _). subst a1. eapply NISStep. intros. rewrite IL in RET. discriminate RET. clear n0.
